---
title: "test"
output: html_document
date: "2023-04-23"
---

```{r}

We have the following equation:
$$\frac{1}{|C_k|} \sum _{i, i^{’} \in C_k} \sum _{j=1}^{p} (x _{ij} - x _{i^{’}j})^2 = 2\sum _{i \in C_k} \sum _{j=1}^{p} (x _{ij} - \bar{x} _{kj})^2 \tag{10.12}$$

Where, $\bar{x} _{kj} = \frac{1}{|C_k|} \sum _{i \in C_k} x _{ij}$ is the mean for feature $j$ in cluster $C_k$.

Expanding the LHS over i:

$$ 
\frac{1}{|C_k|}\sum_{i,i' \in C_k}\sum_{j=1}^p (x_{ij}-x_{i'j})^2 = 
    \frac{1}{|C_k|}\sum_{i' \in C_k}\sum_{j=1}^p (x_{1j}-x_{i'j})^2 + 
    \frac{1}{|C_k|}\sum_{i' \in C_k}\sum_{j=1}^p (x_{2j}-x_{i'j})^2 + ...
$$



Further expanding a single term from the summation:


$$
\begin{aligned}
\frac{1}{|C_k|}\sum_{i' \in C_k,i'\neq i}\sum_{j=1}^p (x_{ij}-x_{i'j})^2 
   &= \frac{1}{|C_k|}\sum_{i' \in C_k,i'\neq i}\sum_{j=1}^p ((x_{ij}-\bar{x}_j)-(x_{i'j}-\bar{x_j}))^2 \\
   &=\frac{1}{|C_k|}\sum_{i' \in C_k,i'\neq i}\sum_{j=1}^p ((x_{ij}-\bar{x}_j)^2-2(x_{ij}-\bar{x}_j)(x_{i'j}-\bar{x_j})+(x_{i'j}-\bar{x_j})^2) \\
   &=\frac{1}{|C_k|}\sum_{i \in C_k}\sum_{j=1}^p (x_{ij}-\bar{x}_j)^2
      -\frac{2}{|C_k|}\sum_{i' \in C_k,i'\neq i}\sum_{j=1}^p(x_{ij}-\bar{x}_j)(x_{i'j}-\bar{x_j}) 
      +\frac{1}{|C_k|}\sum_{i' \in C_k}\sum_{j=1}^p(x_{i'j}-\bar{x_j})^2 \\
   &=\frac{2}{|C_k|}\sum_{i \in C_k}\sum_{j=1}^p (x_{ij}-\bar{x}_j)^2
-\frac{2}{|C_k|}\sum_{i' \in C_k,i'\neq i}\sum_{j=1}^p(x_{ij}-\bar{x}_j)(x_{i'j}-\bar{x_j})
\end{aligned}
$$

Substituting the final term from above in the summation:

$$ 
2\frac{|C_k|}{|C_k|}\sum_{i \in C_k}\sum_{j=1}^p (x_{ij}-\bar{x}_j)^2
\underbrace{-\frac{2}{|C_k|}\sum_{i' \in C_k,i'\neq i}\sum_{j=1}^p(x_{1j}-\bar{x}_j)(x_{i'j}-\bar{x_j})
-\frac{2}{|C_k|}\sum_{i' \in C_k,i'\neq i}\sum_{j=1}^p(x_{2j}-\bar{x}_j)(x_{i'j}-\bar{x_j})+...}_{\text{This term is equal to zero because}\sum_{i' \in C_k}x_{i'j}-|C_k| \bar{x_j}=0}
$$

The remaining term is:

$$
\begin{aligned}
2\frac{|C_k|}{|C_k|}\sum_{i \in C_k}\sum_{j=1}^p (x_{ij}-\bar{x}_j)^2
\qquad\text{Proving 10.12}
\end{aligned}
$$

```
